examples/hoare_logic/blocking_semantics3/blocking_semantics3_WP_monotonicity_4.v
@@ -693,13 +693,16 @@ Axiom abstract_effects_generalize : forall (sigma:(map mident value))
   (pi:(list (ident* value)%type)) (s:stmt) (f:fmla), (eval_fmla sigma pi
   (abstract_effects s f)) -> (eval_fmla sigma pi f).
 
-Axiom abstract_effects_monotonic : forall (s:stmt) (p:fmla),
-  (valid_fmla p) -> (valid_fmla (abstract_effects s p)).
-
-Axiom abstract_effects_monotonic_2 : forall (s:stmt) (p:fmla) (q:fmla),
+Axiom abstract_effects_monotonic : forall (s:stmt) (p:fmla) (q:fmla),
   (valid_fmla (Fimplies p q)) -> forall (sigma:(map mident value)) (pi:(list
   (ident* value)%type)), (eval_fmla sigma pi (abstract_effects s p)) ->
   (eval_fmla sigma pi (abstract_effects s q)).
+
+Axiom abstract_effects_distrib_conj : forall (s:stmt) (p:fmla) (q:fmla)
+  (sigma:(map mident value)) (pi:(list (ident* value)%type)),
+  ((eval_fmla sigma pi (abstract_effects s p)) /\ (eval_fmla sigma pi
+  (abstract_effects s q))) -> (eval_fmla sigma pi (abstract_effects s (Fand p
+  q))).
 
 (* Why3 assumption *)
 Fixpoint wp(s:stmt) (q:fmla) {struct s}: fmla :=
@@ -741,7 +744,7 @@ unfold valid_fmla.
 simpl.
 intros H1 p q H2.
 intuition.
-apply abstract_effects_monotonic_2 with (2:=H3).
+apply abstract_effects_monotonic with (2:=H3).
 unfold valid_fmla; simpl.
 intuition.
 Qed.
